update

Chapter2/Basic.lean
@@ -1,1 +1,48 @@
-def hello := "world"
+import Mathlib.Data.Nat.Basic
+import Mathlib.Tactic
+
+namespace Imp
+
+-- A `State` can be modeled as a function mapping variable names
+-- to values (e.g., natural numbers in this tutorial)
+def State := String -> ℕ
+
+-- Retrive the value of a variable in the State
+def get (st: State) (x : String) : ℕ := st x
+
+-- Update the State with a new value for a variable
+def set (st: State) (x : String) (v: ℕ) : State :=
+  fun y => if y = x then v else st y
+
+-- Syntax of commands
+inductive Command: Type
+| skip: Command                               -- nop
+| assign (x : String) (a: ℕ) : Command        -- x := a
+| assignvar (x: String) (y: String) : Command -- x := y
+| seq (c1 c2 : Command) : Command                 -- c1; c2
+| if_ (b : Bool) (c1 c2 : Command) : Command      -- if b then c1 else c2
+| while (b : Bool) (c : Command) : Command        -- while b do c
+
+-- inductive definitions in Lean come with an important implicit principle:
+-- ** the only ways to construct proofs of the inductive relation are through its constructors.
+
+-- State transition
+inductive CEval : Command -> State -> State -> Prop
+| skip (st : State) :
+    CEval .skip st st
+| assign (st : State) (x : String) (n : ℕ) :
+    CEval (.assign x n) st (set st x n)
+| assignvar (st : State) (x : String) (y : String) :
+    CEval (.assignvar x y) st (set st x (get st y))
+| seq (c1 c2 : Command) (st st' st'' : State) :
+    CEval c1 st st' → CEval c2 st' st'' → CEval (.seq c1 c2) st st''
+| if_true (st st' : State) (c1 c2 : Command) :
+    CEval c1 st st' → CEval (.if_ true c1 c2) st st'
+| if_false (st st' : State) (b : Bool) (c1 c2 : Command) :
+    CEval c2 st st' → CEval (.if_ false c1 c2) st st'
+| while_false (st : State) (c : Command) :
+    CEval (.while false c) st st
+| while_true (st st' st'' : State) (c : Command) :
+    CEval c st st' → CEval (.while true c) st' st'' → CEval (.while true c) st st''
+
+end Imp
