Chapter2/Equiv.lean
@@ -1,67 +1,26 @@
 import Mathlib.Data.Nat.Basic
 import Mathlib.Tactic
-
--- A `State` can be modeled as a function mapping variable names
--- to values (e.g., natural numbers in this tutorial)
-def State := String -> ℕ
-
--- Retrive the value of a variable in the State
-def get (st: State) (x : String) : ℕ := st x
-
--- Update the State with a new value for a variable
-def set (st: State) (x : String) (v: ℕ) : State :=
-  fun y => if y = x then v else st y
-
--- Syntax of commands
-inductive Command: Type
-| skip: Command                               -- nop
-| assign (x : String) (a: ℕ) : Command        -- x := a
-| assignvar (x: String) (y: String) : Command -- x := y
-| seq (c1 c2 : Command) : Command                 -- c1; c2
-| if_ (b : Bool) (c1 c2 : Command) : Command      -- if b then c1 else c2
-| while (b : Bool) (c : Command) : Command        -- while b do c
-
--- inductive definitions in Lean come with an important implicit principle:
--- ** the only ways to construct proofs of the inductive relation are through its constructors.
-
--- State transition
-inductive CEval : Command -> State -> State -> Prop
-| skip (st : State) :
-    CEval .skip st st
-| assign (st : State) (x : String) (n : ℕ) :
-    CEval (.assign x n) st (set st x n)
-| assignvar (st : State) (x : String) (y : String) :
-    CEval (.assignvar x y) st (set st x (get st y))
-| seq (c1 c2 : Command) (st st' st'' : State) :
-    CEval c1 st st' → CEval c2 st' st'' → CEval (.seq c1 c2) st st''
-| if_true (st st' : State) (c1 c2 : Command) :
-    CEval c1 st st' → CEval (.if_ true c1 c2) st st'
-| if_false (st st' : State) (b : Bool) (c1 c2 : Command) :
-    CEval c2 st st' → CEval (.if_ false c1 c2) st st'
-| while_false (st : State) (c : Command) :
-    CEval (.while false c) st st
-| while_true (st st' st'' : State) (c : Command) :
-    CEval c st st' → CEval (.while true c) st' st'' → CEval (.while true c) st st''
+import Chapter2.Basic
 
 namespace Equiv
 
-def cequiv (c₁ c₂ : Command) : Prop :=
-    ∀ (st st' : State),
-    CEval c₁ st st' ↔ CEval c₂ st st'
+def cequiv (c₁ c₂ : Imp.Command) : Prop :=
+    ∀ (st st' : Imp.State),
+    Imp.CEval c₁ st st' ↔ Imp.CEval c₂ st st'
 
--- Executing `skip` does not change the State
+-- Executing `skip` does not change the Imp.State
 -- This directly follows from the `skip` rule
-theorem skip_preserves_State:
-  ∀ (st: State), CEval Command.skip st st := by
-  apply CEval.skip
+theorem skip_preserves_Imp.State:
+  ∀ (st: Imp.State), Imp.CEval Imp.Command.skip st st := by
+  apply Imp.CEval.skip
 
--- Proving a command equivalence
+-- Proving a Imp.Command equivalence
 
 -- ∀c, (skip; c) is equivalent to c
 theorem skip_left:
-  ∀ (c: Command), cequiv (Command.seq Command.skip c) c := by
+  ∀ (c: Imp.Command), cequiv (Imp.Command.seq Imp.Command.skip c) c := by
   intro c
-  -- breaking the Statement into two directions
+  -- breaking the Imp.Statement into two directions
   rw [cequiv]
   intros st st'
   constructor
@@ -71,9 +30,9 @@ theorem skip_left:
     -- This breaks `h` down into its components.
     cases h
     -- This pattern matches the `seq` constructor, giving us:
-    --     `st''`: An intermediate State after executing skip
-    --     `h_skip`: A proof that `CEval Command.skip st st''`
-    --     `h_c`: A proof that `CEval c st'' st'`
+    --     `st''`: An intermediate Imp.State after executing skip
+    --     `h_skip`: A proof that `Imp.CEval Imp.Command.skip st st''`
+    --     `h_c`: A proof that `Imp.CEval c st'' st'`
     case seq st'' h_skip h_c =>
         cases h_skip
         -- Matches the `skip` constructor
@@ -81,12 +40,12 @@ theorem skip_left:
             exact h_c
   -- backward (←)
   . intro h
-    apply CEval.seq
-    . apply CEval.skip
+    apply Imp.CEval.seq
+    . apply Imp.CEval.skip
     . exact h
 
 theorem skip_right:
-    ∀ (c: Command), cequiv (Command.seq c Command.skip) c := by
+    ∀ (c: Imp.Command), cequiv (Imp.Command.seq c Imp.Command.skip) c := by
     intro c
     rw[cequiv]
     intros st st'
@@ -98,12 +57,12 @@ theorem skip_right:
         case skip =>
             exact h_c
     . intro h
-      apply CEval.seq
+      apply Imp.CEval.seq
       . exact h
-      . apply CEval.skip
+      . apply Imp.CEval.skip
 
 theorem if_true:
-    ∀ (b: Bool), ∀ (c₁ c₂ : Command), b = true → cequiv (Command.if_ b c₁ c₂) c₁ := by
+    ∀ (b: Bool), ∀ (c₁ c₂ : Imp.Command), b = true → cequiv (Imp.Command.if_ b c₁ c₂) c₁ := by
     intros b c₁ c₂ htrue
     rw[cequiv]
     intros st st'
@@ -116,11 +75,11 @@ theorem if_true:
         contradiction
     . intro h
       rw[htrue]
-      apply CEval.if_true
+      apply Imp.CEval.if_true
       exact h
 
 theorem if_false:
-    ∀ (b: Bool), ∀ (c₁ c₂ : Command), b = false → cequiv (Command.if_ b c₁ c₂) c₂ := by
+    ∀ (b: Bool), ∀ (c₁ c₂ : Imp.Command), b = false → cequiv (Imp.Command.if_ b c₁ c₂) c₂ := by
     intros b c₁ c₂ hfalse
     rw[cequiv]
     intros st st'
@@ -133,13 +92,13 @@ theorem if_false:
         exact hc
     . intro h
       rw[hfalse]
-      apply CEval.if_false
+      apply Imp.CEval.if_false
       exact b
       exact h
 
 
 theorem swap_if_branches:
-    ∀ (b : Bool), ∀ (c₁ c₂ : Command), cequiv (Command.if_ b c₁ c₂) (Command.if_ (¬b) c₂ c₁) := by
+    ∀ (b : Bool), ∀ (c₁ c₂ : Imp.Command), cequiv (Imp.Command.if_ b c₁ c₂) (Imp.Command.if_ (¬b) c₂ c₁) := by
     intros b c₁ c₂
     rw[cequiv]
     intros st st'
@@ -170,7 +129,7 @@ theorem swap_if_branches:
         repeat rfl
 
 theorem while_false:
-    ∀ (b : Bool), ∀ (c : Command), b = false → cequiv (Command.while b c) Command.skip := by
+    ∀ (b : Bool), ∀ (c : Imp.Command), b = false → cequiv (Imp.Command.while b c) Imp.Command.skip := by
     intros b c₁ hfalse
     rw[cequiv]
     intros st st'
@@ -178,17 +137,17 @@ theorem while_false:
     . intro h
       cases h
       case while_false _ =>
-        apply CEval.skip
+        apply Imp.CEval.skip
       case while_true htrue hc hw =>
         contradiction
     . intro h
       cases h
       case skip =>
         rw[hfalse]
-        apply CEval.while_false
+        apply Imp.CEval.while_false
 
 theorem seq_assoc:
-    ∀ (c₁ c₂ c₃ : Command), cequiv (Command.seq (Command.seq c₁ c₂) c₃) (Command.seq c₁ (Command.seq c₂ c₃)) := by
+    ∀ (c₁ c₂ c₃ : Imp.Command), cequiv (Imp.Command.seq (Imp.Command.seq c₁ c₂) c₃) (Imp.Command.seq c₁ (Imp.Command.seq c₂ c₃)) := by
     intros c₁ c₂ c₃
     rw[cequiv]
     intros st st'
@@ -198,9 +157,9 @@ theorem seq_assoc:
       case seq st'' hs hc =>
         cases hs
         case seq st1 h1 h2 =>
-            apply CEval.seq
+            apply Imp.CEval.seq
             . exact h1
-            apply CEval.seq
+            apply Imp.CEval.seq
             . exact h2
             . exact hc
     . intro h
@@ -208,15 +167,15 @@ theorem seq_assoc:
       case seq st'' hs hc =>
         cases hc
         case seq st1 h1 h2 =>
-            apply CEval.seq
-            apply CEval.seq
+            apply Imp.CEval.seq
+            apply Imp.CEval.seq
             .exact hs
             .exact h1
             .exact h2
 
-lemma h_eq (st: State) (x : String) : set st x (get st x) = st := by
+lemma h_eq (st: Imp.State) (x : String) : Imp.set st x (Imp.get st x) = st := by
     funext y
-    unfold _root_.set _root_.get
+    unfold Imp.set Imp.get
     by_cases h: y = x
     {
         rw[if_pos h]
